Alexander.thy
@@ -1,0 +1,238 @@
+
+theory Alexander
+  imports 
+    Simplicial_complex
+begin
+
+context simplicial_complex
+begin
+
+abbreviation "univ_n == {..<n}"
+
+definition simplex_complement
+  where "simplex_complement s == univ_n - s"
+
+subsubsection \<open>Set complement\<close>
+
+lemma
+  simplex_complement_simplex:
+  assumes v: "v \<in> simplices"
+  shows "simplex_complement v \<in> simplices"
+  using v
+  by (simp add: atLeast0LessThan simplex_complement_def simplices_def)
+
+lemma
+  simplex_Compl_in:
+  assumes s: "s \<in> simplices" and c: "c \<in> s"
+  shows "c \<notin> simplex_complement s"
+  using s c
+  unfolding simplices_def 
+  unfolding simplex_complement_def by simp
+
+lemma
+  simplex_Compl_notin:
+  assumes s: "s \<in> simplices" and c: "c \<in> simplex_complement s"
+  shows "c \<notin> s"
+  using s c 
+  unfolding simplices_def 
+  unfolding simplex_complement_def by simp
+
+lemma
+  simplex_Compl_iff [simp]:
+  assumes s: "s \<in> simplices" and c: "c < n"
+  shows "c \<in> simplex_complement s \<longleftrightarrow> c \<notin> s"
+  unfolding simplex_complement_def
+  using s c unfolding simplices_def by simp
+
+lemma
+  assumes "x \<in> simplices"
+  shows "x = simplex_complement (simplex_complement x)"
+  using assms atLeast0LessThan simplex_complement_def simplices_def by auto
+
+lemma
+  simplice_complement:
+  assumes "x \<in> simplices"
+  obtains vx where "x = simplex_complement vx"
+proof -
+  have "simplex_complement (simplex_complement x) = x"
+    using assms atLeast0LessThan simplex_complement_def simplices_def by auto
+  then show ?thesis
+    using that by blast 
+qed
+
+text\<open>We define the complement or the ``no faces'' of a simplicial complex
+  as the set of simplices that is not in the simplicial complex.
+  Note that the set obtained is not a simplicial complex (except 
+  for particular cases such as the empty set or the total set).\<close>
+
+definition nofaces_simplicial_complex
+  where "nofaces_simplicial_complex s = {v. v \<in> simplices \<and> v \<notin> s}"
+
+lemma simpl_compl_not_in [simp]:
+  assumes "v \<in> nofaces_simplicial_complex s" 
+  shows "v \<notin> s"
+  using assms nofaces_simplicial_complex_def by fastforce
+
+lemma simpl_compl_simplice [simp]:
+  assumes "v \<in> nofaces_simplicial_complex s" 
+  shows "v \<in> simplices"
+  by (metis (no_types, lifting) assms mem_Collect_eq nofaces_simplicial_complex_def)
+
+definition Alexander_dual
+  where "Alexander_dual s = 
+            {v. \<exists>x. v = simplex_complement x \<and> x \<in> nofaces_simplicial_complex s}"
+
+lemma
+  simplicial_complex_Alexander_dual:
+  assumes "simplicial_complex s"
+  shows "simplicial_complex (Alexander_dual s)"
+proof (unfold simplicial_complex_def, standard, intro conjI)
+  fix \<sigma> :: "nat set"
+  assume sigma: "\<sigma> \<in> Alexander_dual s"
+  show sigma_simplice: "\<sigma> \<in> simplices"
+    using sigma unfolding Alexander_dual_def using simplex_complement_simplex [OF ]
+    by fastforce
+  show "Pow \<sigma> \<subseteq> Alexander_dual s"
+  proof
+    fix x :: "nat set"
+    assume x: "x \<in> Pow \<sigma>"
+    show "x \<in> Alexander_dual s"
+    proof (rule ccontr)
+      assume xnin: "x \<notin> Alexander_dual s"
+      from x have x_in_sigma: "x \<subseteq> \<sigma>" and x_simplice: "x \<in> simplices" 
+        using sigma_simplice
+        apply simp
+        using sigma_simplice simplices_def x by force
+      from sigma obtain v
+        where sigma_complement: "\<sigma> = simplex_complement v" 
+          and v_noface: "v \<in> nofaces_simplicial_complex s"
+        unfolding Alexander_dual_def by auto
+      from x_simplice
+      obtain vx where x_complement: "x = simplex_complement vx" and vx_simplice: "vx \<in> simplices"
+        using simplice_complement [OF x_simplice]
+        using simplex_complement_simplex [OF x_simplice]
+        by (metis PowD Pow_top atLeast0LessThan double_diff simplex_complement_def simplices_def)
+      show False
+      proof (cases "vx \<in> nofaces_simplicial_complex s")
+        case True
+        hence "x \<in> Alexander_dual s" using x_complement unfolding Alexander_dual_def by auto
+        thus ?thesis using xnin by contradiction
+      next
+        case False
+        hence vx_in_s: "vx \<in> s"
+          by (metis (mono_tags, lifting) mem_Collect_eq nofaces_simplicial_complex_def vx_simplice) 
+        have "v \<subseteq> vx"
+          using sigma_complement x_complement x_in_sigma
+          by (smt (verit, ccfv_threshold) Diff_iff PowD atLeast0LessThan simplices_def simplicial_complex.simpl_compl_simplice simplicial_complex.simplex_complement_def subset_eq v_noface)
+        hence "v \<in> s" using assms vx_in_s unfolding simplicial_complex_def by auto
+        thus ?thesis using v_noface by simp
+      qed
+    qed
+  qed
+qed
+
+end
+
+context boolean_functions
+begin
+
+text\<open>The notion of @{const simplicial_complex.nofaces_simplicial_complex} 
+  in simplicial complexes becomes now in boolean functions just the 
+  @{const HOL.Not} boolean operator.\<close>
+
+(*definition nofaces_boolean_function
+  where "nofaces_boolean_function f = {b. b \<in> carrier_vec n \<and> \<not> f b}"
+
+lemma nofaces_not [simp]:
+  assumes "b \<in> nofaces_boolean_function f"
+  shows "\<not> f b"
+  using assms nofaces_boolean_function_def by fastforce
+
+lemma nofaces_carrier_vec [simp]:
+  assumes "b \<in> nofaces_boolean_function f"
+  shows "b \<in> carrier_vec n"
+  using assms nofaces_boolean_function_def by auto
+
+lemma "nofaces_boolean_function f \<union> {b. b \<in> carrier_vec n \<and> f b} 
+  = carrier_vec n"
+  unfolding nofaces_boolean_function_def by auto*)
+
+text\<open>The notion of @{const simplicial_complex.simplex_complement}
+  becomes now in boolean functions the negation, or the complement in base 
+  @{term "2::nat"}, of each @{typ "bool vec"}.}\<close>
+
+definition not :: "bool vec \<Rightarrow> bool vec"  (*"\<not> _" [20] 20*)
+  where "not v = vec (dim_vec v) (\<lambda>n. \<not> v $ n)"
+
+lemma
+  dim_vec_not:
+  assumes d: "dim_vec v = k"
+  shows "dim_vec (not v) = k"
+  using d unfolding not_def by simp
+
+lemma
+  assumes d: "k < dim_vec v"
+  shows "v $ k \<longleftrightarrow> \<not> (not v $ k)"
+  using d unfolding not_def by simp
+
+lemma
+  not_v_in_carrier:
+  assumes "v \<in> carrier_vec k"
+  shows "not v \<in> carrier_vec k"
+  using assms not_def by fastforce
+
+lemma
+  assumes d: "k < dim_vec v"
+  shows "\<not> v $ k \<longleftrightarrow> (not v $ k)"
+  using d unfolding not_def by simp
+
+text\<open>The operation @{const not} is ``antimonotone'', in the sense that
+  for every @{term x}, @{term y} such that @{term "x \<le> y"}, 
+  then @{term "not y \<le> not x"}.\<close>
+
+lemma
+  not_vec_antimono: 
+  assumes rs: "r \<le> s"
+  shows "not s \<le> not r"
+  using rs 
+  unfolding not_def
+  unfolding less_eq_vec_def by auto
+
+text\<open>The operation @{const HOL.Not} is ``antimonotone'', in the sense that
+  for every @{term x}, @{term y} such that @{term "x \<le> y"},
+  and @{term f} such that @{term "monotone_bool_fun f"},
+  then @{term "HOL.Not (f y) \<le> HOL.Not (f x)"}.\<close>
+
+lemma
+  not_antimono:
+  assumes m: "monotone_bool_fun f"
+  and x: "x \<in> carrier_vec n" and y: "y \<in> carrier_vec n"
+  and xy: "x \<le> y"
+  shows "(\<not> f y) \<le> (\<not> f x)"
+  by (metis (mono_tags, hide_lams) le_boolE le_boolI' m mono_on_def monotone_bool_fun_def x xy y)
+
+text\<open>The definition of the Alexander dual now for a Boolean function @{term f}
+  becomes just the negation of @{term f} over the ``complement'' of every vector.\<close>
+
+definition "Alexander_dual f = (\<lambda>x. \<not> f (not x))"
+
+lemma
+  monotone_boolean_function_Alexander_dual:
+  assumes f: "monotone_bool_fun f"
+  shows "monotone_bool_fun (Alexander_dual f)"
+proof (unfold monotone_bool_fun_def, unfold mono_on_def, intro allI, safe)
+  fix r s :: "bool vec"
+  assume r: "r \<in> carrier_vec n" and s: "s \<in> carrier_vec n" and r_le_s: "r \<le> s"
+  have nr: "not r \<in> carrier_vec n" and ns: "not s \<in> carrier_vec n" and ns_le_nr: "not s \<le> not r"
+    using not_v_in_carrier [OF r]
+        and not_v_in_carrier [OF s] 
+        and not_vec_antimono [OF r_le_s] by simp_all
+  show "Alexander_dual f r \<le> Alexander_dual f s"
+    unfolding Alexander_dual_def using not_antimono [OF f ns nr ns_le_nr] by simp
+qed
+
+end
+
+lemmas [code] = boolean_functions.not_def boolean_functions.Alexander_dual_def
+
+end
